Implement Network.Executable.apply.container

Runtime/Network/Execution/Apply.lean
@@ -1,100 +1,24 @@
-import Runtime.Network.Execution.Basic
+import Runtime.Network.Execution.ReactionOutput
 
-open Network
+namespace Network.Executable
 
-structure Reaction.Output (exec : Executable net) where
-  reactor : ReactorId net
-  reaction : reactor.class.reactionType
-  raw : reaction.outputType exec.tag.time
-
-abbrev Reaction.Output.domain (output : Reaction.Output exec) : Interface.Scheme :=
-  output.reactor.class.interface .outputs
-
-variable {exec : Executable net}
-
-def Reaction.Output.fromRaw {reactor : ReactorId net} {reaction : reactor.class.reactionType} (raw : reaction.outputType exec.tag.time) : Reaction.Output exec :=
-  { reactor, reaction, raw }
-
-def Reaction.Output.events (output : Reaction.Output exec) :=
-  output.raw.events.map fun event => Event.action event.time ⟨output.reactor, event.action⟩ event.value
-
-inductive Reaction.Output.LocalValue (output : Reaction.Output exec) (port : output.domain.vars)
-  | independent
-  | absent
-  | present (value : output.domain.type port)
-
-inductive Reaction.Output.NestedValue (output : Reaction.Output exec) (port : output.domain.vars)
-  | independent
-  | absent
-  | present (value : output.domain.type port) 
-
-def Reaction.Output.LocalValue.value? : LocalValue output port → Option (output.domain.type port)
-  | present value        => value
-  | independent | absent => none
-
--- Note: This theorem is really only needed for `Reaction.Output.local`.
-private def Reaction.Output.local_type_correctness {port'} : 
-  (output.reaction.portEffectsInjCoe.inv (.inl port) = some port') → 
-  (output.reactor.class.reactionOutputScheme |>.restrict output.reaction.portEffects |>.type port') = (domain output).type port :=
-  (by rw [Interface.Scheme.restrict_type, output.reaction.portEffectsInjCoe.invCoeId _ ·])
-
-def Reaction.Output.local (output : Reaction.Output exec) (port : output.domain.vars) : LocalValue output port := 
-  match h : output.reaction.portEffectsInjCoe.inv (.inl port) with
-  | none => .independent
-  | some port' =>
-    match output.raw.ports port' with
-    | none => .absent
-    | some value => .present (local_type_correctness h ▸ value)
-
-theorem Reaction.Output.events_LawfulQueue (output : Reaction.Output exec) : Executable.LawfulQueue output.events exec.tag.time := by
-  intro event h
-  simp [events, Array.map_getElem?, Bind.bind, Option.bind] at h
-  split at h
-  · contradiction
-  case _ e _ => 
-    simp at h
-    simp [Event.time, ←h, e.time.property]
-
-namespace Network.Executable    
-
-def apply (exec : Executable net) (output : Reaction.Output exec) : Executable net := { exec with
+def apply (exec : Executable net) (output : ReactionOutput exec) : Executable net := { exec with
   queue := exec.queue.merge output.events
   reactors := fun id => { exec.reactors id with
     interface := 
-      if      h : id = output.reactor then h ▸ targetReactor output  -- Updates the output ports of the reaction's reactor.
-      else if h : id ≻ output.reactor then nestedReactor output id h -- Updates the input ports of nested reactors.
-      else                                 exec.reactors id |>.interface  -- Unaffected reactors.
+      if      h : id = output.reactor then h ▸ container output -- Updates the output ports of the reaction's container.
+      else if h : id ≻ output.reactor then child output ⟨id, h⟩ -- Updates the input ports of child reactors.
+      else                                 exec.interface id    -- Unaffected reactors.
   }
   lawfulQueue := LawfulQueue.merge exec.lawfulQueue output.events_LawfulQueue
 }
 where 
-  targetReactor (output : Reaction.Output exec) : (kind : Reactor.InterfaceKind) → kind.interfaceType (output.reactor.class.interface kind)
+  container (output : ReactionOutput exec) : (kind : Reactor.InterfaceKind) → kind.interfaceType (output.reactor.class.interface kind)
     | .outputs => fun var => (output.local var).value?.orElse (fun _ => exec.interface output.reactor .outputs var)
     | .state => output.raw.state
-    | interface => exec.interface output.reactor interface
-  nestedReactor (output : Reaction.Output exec) (id : ReactorId net) (hc : id ≻ output.reactor) : (kind : Reactor.InterfaceKind) → kind.interfaceType (id.class.interface kind)
-    | .inputs => sorry -- nestedInputs exec output id hc
-    | interface => exec.reactors id |>.interface interface 
-  -- nestedInputs (exec : Executable net) (output : Reaction.Output net) (id : ReactorId net) (hc : id ≻ output.reactor) : Interface? (id.class.interface .inputs) :=
-  --  let currentReactor := exec.reactors id
-  --  fun var =>
-      /-
-      let nestedID := id.last hc
-      have h₁ : (net.scheme id |>.interface .inputs).vars = (net.subinterface (net.class reactorID) nestedID .inputs).vars := by sorry -- rw [Graph.child_schemes_eq_parent_subschemes]
-      let var₁ : (net.reactionOutputScheme' reactorID).vars := .inr ⟨nestedID, h₁ ▸ var⟩
-      match h : InjectiveCoe.inv var₁ with 
-      | none => currentReactor.interface .inputs var
-      | some var₂ =>
-        match output.ports var₂ with
-        | none => currentReactor.interface .inputs var
-        | some val =>
-          have h : (net.class reactorID |> net.reactionOutputScheme |>.restrict reaction.portEffects).type var₂ = (net.scheme id |>.interface .inputs).type var := by
-            rw [(net.reactionOutputScheme' reactorID).restrict_type]
-            rw [InjectiveCoe.invCoeId _ h]
-            -- have := Graph.child_schemes_eq_parent_subschemes hc
-            sorry
-          h ▸ val
-      -/
+    | _ => exec.interface output.reactor _
+  child (output : ReactionOutput exec) (id : ReactorId.Child output.reactor) : (kind : Reactor.InterfaceKind) → kind.interfaceType ((id : ReactorId net).class.interface kind)
+    | .inputs => fun var => (output.child var).value?.orElse (fun _ => exec.interface id .inputs var)
+    | _ => exec.interface id _
 
-
-end Network.Executable    
+end Network.Executable
