Runtime/Network/Basic.lean
@@ -16,6 +16,19 @@ def Graph.Class.connections {net : Network} (cls : Class net) := net.connections
 
 abbrev ReactorId (net : Network) := Graph.Path net net.root
 
+abbrev ReactorId.inputs (reactor : ReactorId net) :=
+  reactor.class.interface .inputs
+
+abbrev ReactorId.outputs (reactor : ReactorId net) :=
+  reactor.class.interface .outputs
+
+abbrev ReactorId.Child (reactor : ReactorId net) :=
+  { child : ReactorId net // child ≻ reactor }
+
+-- TODO: This should probably be a more general property on Graph.Path
+def ReactorId.Child.class (child : Child reactor) : Graph.Class.Child reactor.class where
+  id := sorry -- child.val.class 
+
 structure ActionId (net : Network) where
   reactor : ReactorId net
   action : (reactor.class.interface .actions).vars
