Runtime/Network/Execution/ReactionOutput.lean
@@ -1,0 +1,85 @@
+import Runtime.Network.Execution.Basic
+
+namespace Network.Executable
+
+structure ReactionOutput (exec : Executable net) where
+  reactor : ReactorId net
+  reaction : reactor.class.reactionType
+  raw : reaction.outputType exec.tag.time
+
+namespace ReactionOutput
+
+variable {exec : Executable net}
+
+def fromRaw {reactor : ReactorId net} {reaction : reactor.class.reactionType} (raw : reaction.outputType exec.tag.time) : ReactionOutput exec :=
+  { reactor, reaction, raw }
+
+def events (output : ReactionOutput exec) :=
+  output.raw.events.map fun event => Event.action event.time ⟨output.reactor, event.action⟩ event.value
+
+inductive Value (α : Type)
+  | independent
+  | absent
+  | present (value : α)
+
+def Value.value? : Value α → Option α
+  | present value        => value
+  | independent | absent => none
+
+-- Note: This theorem is really only needed for `Reaction.Output.local`.
+private def local_type_correctness {output : ReactionOutput exec} {port port'} : 
+  (output.reaction.portEffectsInjCoe.inv (.inl port) = some port') → 
+  (output.reactor.class.reactionOutputScheme |>.restrict output.reaction.portEffects |>.type port') = output.reactor.outputs.type port :=
+  (by rw [Interface.Scheme.restrict_type, output.reaction.portEffectsInjCoe.invCoeId _ ·])
+
+def «local» (output : ReactionOutput exec) (port : output.reactor.outputs.vars) : Value (output.reactor.outputs.type port) := 
+  match h : output.reaction.portEffectsInjCoe.inv (.inl port) with
+  | none => .independent
+  | some port' =>
+    match output.raw.ports port' with
+    | none => .absent
+    | some value => .present (local_type_correctness h ▸ value)
+
+def child (output : ReactionOutput exec) {child : ReactorId.Child output.reactor} (port : (child : ReactorId net).inputs.vars) : Value ((child : ReactorId net).inputs.type port) := 
+  -- match h : output.reaction.portEffectsInjCoe.inv (.inr ⟨child.class, port⟩) with
+  -- | none => .independent
+  -- | some port' =>
+  --   match output.raw.ports port' with
+  --   | none => .absent
+  --   | some value => .present (local_type_correctness h ▸ value)
+  sorry
+    -- nestedInputs (exec : Executable net) (output : Reaction.Output net) (id : ReactorId net) (hc : id ≻ output.reactor) : Interface? (id.class.interface .inputs) :=
+  --  let currentReactor := exec.reactors id
+  --  fun var =>
+      /-
+      let nestedID := id.last hc
+      have h₁ : (net.scheme id |>.interface .inputs).vars = (net.subinterface (net.class reactorID) nestedID .inputs).vars := by sorry -- rw [Graph.child_schemes_eq_parent_subschemes]
+      let var₁ : (net.reactionOutputScheme' reactorID).vars := .inr ⟨nestedID, h₁ ▸ var⟩
+      match h : InjectiveCoe.inv var₁ with 
+      | none => currentReactor.interface .inputs var
+      | some var₂ =>
+        match output.ports var₂ with
+        | none => currentReactor.interface .inputs var
+        | some val =>
+          have h : (net.class reactorID |> net.reactionOutputScheme |>.restrict reaction.portEffects).type var₂ = (net.scheme id |>.interface .inputs).type var := by
+            rw [(net.reactionOutputScheme' reactorID).restrict_type]
+            rw [InjectiveCoe.invCoeId _ h]
+            -- have := Graph.child_schemes_eq_parent_subschemes hc
+            sorry
+          h ▸ val
+      -/
+
+
+
+
+theorem events_LawfulQueue (output : ReactionOutput exec) : Executable.LawfulQueue output.events exec.tag.time := by
+  intro _ h
+  simp [events, Array.map_getElem?, Bind.bind, Option.bind] at h
+  split at h
+  · contradiction
+  case _ e _ => 
+    simp at h
+    simp [Event.time, ←h, e.time.property]
+
+end ReactionOutput
+end Network.Executable
